lib/partialmap.fst
@@ -1,25 +1,91 @@
-module PartialMap
+module Map
 open Prims.PURE
-
 assume type t : Type -> Type -> Type
+type set (a:Type) = t a bool
+assume logic val sel :       key:Type -> value:Type -> t key value -> key -> Tot value
+assume logic val upd :       key:Type -> value:Type -> t key value -> key -> value -> Tot (t key value)
+assume logic val const :     key:Type -> value:Type -> v:value -> Tot (t key value)
+assume logic val concat:     key:Type -> value:Type -> t key value -> t key value -> Tot (t key value)
+assume logic val contains:   key:Type -> value:Type -> t key value -> key -> Tot bool
+assume logic val equal:      key:Type -> value:Type -> t key value -> t key value -> Tot bool
+assume logic val intersect:  key:Type -> set key -> set key -> Tot (set key)
+assume logic val complement: key:Type -> set key -> Tot (set key)
+assume logic val restrict:   key:Type -> value:Type -> set key -> t key value -> Tot (t key value)
 
-assume logic val Sel : 'k:Type -> 'v:Type -> m:t 'k 'v -> k:'k -> Tot 'v
-assume logic val Upd : 'k:Type -> 'v:Type -> m:t 'k 'v -> k:'k -> v:'v -> Tot (t 'k 'v)
-assume logic val Emp : 'k:Type -> 'v:Type -> Tot (t 'k 'v)
-assume logic val Concat: 'k:Type -> 'v:Type -> t 'k 'v -> t 'k 'v -> Tot (t 'k 'v)
-assume logic val ConstMap: 'k:Type -> 'v:Type -> set 'k -> 'v -> Tot (t 'k 'v)
-logic type InDom  : #'k:Type -> #'v:Type -> 'k -> t 'k 'v -> Type
-logic type DisjointDom ('k:Type) ('v:Type) (m1:t 'k 'v) (m2:t 'k 'v) = 
-          (forall x.{:pattern (InDom x m1)} InDom x m1 ==> ~(InDom x m2))
-                         
-assume SelUpd1: forall ('k:Type) ('v:Type) (m:t 'k 'v) (k:'k) (v:'v).{:pattern (Sel (Upd m k v) k)} Sel (Upd m k v) k == k
-assume SelUpd2: forall ('k:Type) ('v:Type) (m:t 'k 'v) (k1:'k) (k2:'k) (v:'v).{:pattern (Sel (Upd m k2 v) k1)} k2=!=k1 ==> Sel (Upd m k2 v) k1 == Sel m k1
-assume SelConst: forall ('k:Type) ('v:Type) (keys:set 'k) (v:'v) (k:'k).{:pattern (Sel (ConstMap keys v) k)} InSet k keys ==> Sel (ConstMap keys v) k == v
-(* assume InDomEmp:   forall ('k:Type) ('v:Type) (kk:'k).{:pattern InDom 'k 'v kk (Emp 'k 'v)} ~(InDom 'k 'v kk (Emp 'k 'v)) *)
-assume InDomUpd1:     forall ('k:Type) ('v:Type) (m:t 'k 'v) (k:'k) (v:'v).{:pattern InDom k (Upd m k v)} InDom k (Upd m k v)
-assume InDomUpd2:     forall ('k:Type) ('v:Type) (m:t 'k 'v) (k1:'k) (k2:'k) (v:'v).{:pattern InDom k1 (Upd m k2 v)} (k2=!=k1 /\ InDom k1 m) ==> InDom k1 (Upd m k2 v)
-assume InDomConstMap: forall ('k:Type) ('v:Type) (keys:set 'k) (v:'v) (k:'k).{:pattern InDom k (ConstMap keys v)} InDom k (ConstMap keys v) <==> InSet k keys
-assume InDomConcat:   forall ('k:Type) ('v:Type) (m1:t 'k 'v) (m2:t 'k 'v) (k:'k).{:pattern InDom k (Concat m1 m2)} InDom k (Concat m1 m2) <==> (InDom k m1 \/ InDom k m2)
-assume SelConcat1: forall ('k:Type) ('v:Type) (m1:t 'k 'v) (m2:t 'k 'v) (k:'k).{:pattern Sel (Concat m1 m2) k} InDom k m2 ==> Sel (Concat m1 m2) k==Sel m2 k
-assume SelConcat1: forall ('k:Type) ('v:Type) (m1:t 'k 'v) (m2:t 'k 'v) (k:'k).{:pattern Sel (Concat m1 m2) k} ~(InDom k m2) ==> Sel (Concat m1 m2) k==Sel m1 k
+assume SelUpd1:       forall (key:Type) (value:Type) (m:t key value) (k:key) (v:value).          {:pattern (sel (upd m k v) k)}        sel (upd m k v) k == v
+assume SelUpd2:       forall (key:Type) (value:Type) (m:t key value) (k1:key) (k2:key) (v:value).{:pattern (sel (upd m k2 v) k1)}      k2=!=k1 ==> sel (upd m k2 v) k1 == sel m k1
+assume SelConst:      forall (key:Type) (value:Type) (v:value) (k:key).                          {:pattern (sel (const v) k)}          sel (const v) k == v
+assume SelRestrict:   forall (key:Type) (value:Type) (m:t key value) (ks:set key) (k:key).       {:pattern (sel (restrict ks m) k)}    sel ks k ==> sel (restrict ks m) k == sel m k
+assume SelConcat1:    forall (key:Type) (value:Type) (m1:t key value) (m2:t key value) (k:key).  {:pattern sel (concat m1 m2) k}       contains m2 k ==> sel (concat m1 m2) k==sel m2 k
+assume SelConcat1:    forall (key:Type) (value:Type) (m1:t key value) (m2:t key value) (k:key).  {:pattern sel (concat m1 m2) k}       not(contains m2 k) ==> sel (concat m1 m2) k==sel m1 k
+
+assume InDomUpd1:     forall (key:Type) (value:Type) (m:t key value) (k:key) (v:value).          {:pattern contains (upd m k v) k}     contains (upd m k v) k
+assume InDomUpd2:     forall (key:Type) (value:Type) (m:t key value) (k1:key) (k2:key) (v:value).{:pattern contains (upd m k2 v) k1}   k2=!=k1 ==> contains (upd m k2 v) k1 == contains m k1
+assume InDomConstMap: forall (key:Type) (value:Type) (v:value) (k:key).                          {:pattern contains (const v) k}       contains (const v) k
+assume InDomConcat:   forall (key:Type) (value:Type) (m1:t key value) (m2:t key value) (k:key).  {:pattern contains (concat m1 m2) k}  contains (concat m1 m2) k==(contains m1 k || contains m2 k)
+assume InDomRestrict: forall (key:Type) (value:Type) (m:t key value) (ks:set key) (k:key).       {:pattern contains (restrict ks m) k} contains (restrict ks m) k == sel ks k
+assume ContainsConst: forall (key:Type) (value:Type) (v:value) (k:key).                          {:pattern contains (const v) k}       not (contains (const v) k)
+
+assume InInter:       forall (key:Type) (s1:set key) (s2:set key) (k:key).                       {:pattern sel (intersect s1 s2) k}    sel (intersect s1 s2) k == (sel s1 k && sel s2 k)
+assume InComplement:  forall (key:Type) (s:set key) (k:key).                                     {:pattern sel (complement s) k}       sel (complement s) k == not (sel s k)
+assume Extensional:   forall (key:Type) (value:Type) (m1:t key value) (m2:t key value).          {:pattern (equal m1 m2)}              equal m1 m2 <==> m1 == m2
+assume Equals:        forall (key:Type) (value:Type) (m1:t key value) (m2:t key value).          {:pattern (equal m1 m2)}              equal m1 m2 <==> (forall k.{:pattern (sel m1 k); (sel m2 k)} sel m1 k == sel m2 k)
+
+
+let const_on (key:Type) (value:Type) (dom:set key) (v:value) = restrict dom (const v) 
+
+opaque type DisjointDom (key:Type) (value:Type) (m1:t key value) (m2:t key value) = 
+          (forall x.{:pattern (contains m1 x)(* ; (contains m2 x) *)} contains m1 x ==> not (contains m2 x))
+
+module Set
+open Map
+type set (a:Type) = Map.t a bool
+let empty      (a:Type)                        = const a bool false
+let singleton  (a:Type) (x:a)                  = upd empty x true
+let mem        (a:Type) (x:a)      (s:set a)   = sel s x
+let union      (a:Type) (s1:set a) (s2:set a)  = concat s1 s2
+let intersect  (a:Type) (s1:set a) (s2:set a)  = intersect s1 s2
+let extend     (a:Type) (k:a)      (s:set a)   = upd s k true
+let complement (a:Type) (s:set a)              = complement s
+let minus      (a:Type) (s1:set a) (s2:set a)  = intersect s1 (complement s2)
+let equal      (a:Type) (s1:set a) (s2:set a)  = Map.equal s1 s2
+opaque type Subset' (a:Type) (s1:set a) (s2:set a) = (forall (x:a).{:pattern mem x s1} mem x s1 ==> mem x s2)
+type Subset : #a:Type -> set a -> set a -> Type = 
+    fun (a:Type) (s1:set a) (s2:set a) -> Subset' a s1 s2
+
+module Heap
+open Set
+
+type aref = 
+  | Ref : a:Type -> r:ref a -> aref
+
+type refs =
+  | AllRefs : refs
+  | SomeRefs : v:set aref -> refs
+
+let no_refs  = SomeRefs empty
+let a_ref  r = SomeRefs (singleton (Ref r))
+
+assume logic val sel :       a:Type -> heap -> ref a -> Tot a
+assume logic val upd :       a:Type -> heap -> ref a -> a -> Tot heap
+assume logic val emp :       heap
+assume logic val contains :  a:Type -> heap -> ref a -> Tot bool
+assume logic val equal:      heap -> heap -> Tot bool
+assume logic val restrict:   heap -> set aref -> Tot heap
+assume logic val concat:     heap -> heap -> Tot heap
+
+assume SelUpd1:       forall (a:Type) (h:heap) (r:ref a) (v:a).            {:pattern (sel (upd h r v) r)}       sel (upd h r v) r == v
+assume SelUpd2:       forall (a:Type) (h:heap) (k1:ref a) (k2:ref a) (v:a).{:pattern (sel (upd h k2 v) k1)}     k2=!=k1 ==> sel (upd h k2 v) k1 == sel h k1
+assume InDomUpd1:     forall (a:Type) (h:heap) (k:ref a) (v:a).            {:pattern contains (upd h k v) k}    contains (upd h k v) k
+assume InDomUpd2:     forall (a:Type) (h:heap) (k1:ref a) (k2:ref a) (v:a).{:pattern contains (upd h k2 v) k1}  k2=!=k1 ==> contains (upd h k2 v) k1 == contains h k1
+assume InDomEmp:      forall (a:Type) (k:ref a).                           {:pattern contains emp k}            not(contains emp k)
+assume Extensional:   forall (h1:heap) (h2:heap).                          {:pattern equal h1 h2}               equal h1 h2 <==> h1 == h2
+assume Equals:        forall (h1:heap) (h2:heap).                          {:pattern equal h1 h2}               equal h1 h2 <==> (forall (a:Type) (k:ref a).{:pattern (sel h1 k); (sel h2 k)} sel h1 k == sel h2 k)
+assume RestrictSel:   forall (a:Type) (h:heap) (r:set aref) (a:ref a).     {:pattern sel (restrict h r) a}      if b2t (mem (Ref a) r) then sel (restrict h r) a == sel h a else sel (restrict h r) a == sel emp a 
+assume RestrictIn:    forall (a:Type) (h:heap) (r:set aref) (a:ref a).     {:pattern contains (restrict h r) a} contains (restrict h r) a == (mem (Ref a) r && contains h a)
+assume SelConcat:     forall (a:Type) (h1:heap) (h2:heap) (a:ref a).       {:pattern sel (concat h1 h2) a}      if b2t (contains h2 a) then sel (concat h1 h2) a==sel h2 a else sel (concat h1 h2) a == sel h1 a
+assume ContainsConcat:forall (a:Type) (h1:heap) (h2:heap) (a:ref a).       {:pattern contains (concat h1 h2) a} contains h1 a || contains h2 a
+
+type On (r:set aref) (p:(heap -> Type)) (h:heap) = p (restrict h r)
+opaque type fresh (h:heap) (refs:set aref)       = (forall (a:Type) (a:ref a).{:pattern (contains h a)} mem (Ref a) refs ==> not(contains h a))
 
